compiler/backend/semantics/stackPropsScript.sml
@@ -318,6 +318,16 @@ val inst_clock_neutral = prove(
   \\ full_simp_tac(srw_ss())[mem_load_def,get_var_def,mem_store_def]
   \\ srw_tac[][state_component_equality]);
 
+val inst_clock_neutral_ffi = prove(
+  ``(inst i s = SOME t ==> inst i (s with ffi := k) = SOME (t with ffi := k)) /\
+    (inst i s = NONE ==> inst i (s with ffi := k) = NONE)``,
+  Cases_on `i` \\ full_simp_tac(srw_ss())[inst_def,assign_def,word_exp_def,set_var_def,LET_DEF]
+  \\ rpt (srw_tac[][state_component_equality]
+  \\ every_case_tac \\ full_simp_tac(srw_ss())[] \\ srw_tac[][] \\ full_simp_tac(srw_ss())[word_exp_def]
+  \\ every_case_tac \\ full_simp_tac(srw_ss())[] \\ srw_tac[][] \\ full_simp_tac(srw_ss())[word_exp_def]
+  \\ full_simp_tac(srw_ss())[mem_load_def,get_var_def,mem_store_def]
+  \\ srw_tac[][state_component_equality]));
+
 val evaluate_clock_neutral = store_thm("evaluate_clock_neutral",
   ``!prog s res t.
       evaluate (prog,s) = (res,t) /\ clock_neutral prog ==>
@@ -328,6 +338,19 @@ val evaluate_clock_neutral = store_thm("evaluate_clock_neutral",
   THEN1 (every_case_tac \\ imp_res_tac inst_clock_neutral \\ full_simp_tac(srw_ss())[])
   THEN1 (Cases_on `evaluate (c1,s)` \\ full_simp_tac(srw_ss())[LET_THM] \\ every_case_tac \\ full_simp_tac(srw_ss())[])
   \\ `get_var_imm ri (s with clock := c) = get_var_imm ri s` by
+         (Cases_on `ri` \\ full_simp_tac(srw_ss())[get_var_imm_def,get_var_def])
+  \\ every_case_tac \\ full_simp_tac(srw_ss())[] \\ srw_tac[][] \\ full_simp_tac(srw_ss())[set_var_def]);
+
+val evaluate_ffi_neutral = store_thm("evaluate_ffi_neutral",
+  ``!prog s res t.
+      evaluate (prog,s) = (res,t) /\ clock_neutral prog ==>
+      evaluate (prog,s with ffi := c) = (res,t with ffi := c)``,
+  recInduct evaluate_ind \\ srw_tac[][] \\ full_simp_tac(srw_ss())[]
+  \\ full_simp_tac(srw_ss())[evaluate_def,get_var_def,clock_neutral_def]
+  THEN1 (every_case_tac \\ full_simp_tac(srw_ss())[] \\ srw_tac[][] \\ full_simp_tac(srw_ss())[empty_env_def])
+  THEN1 (every_case_tac \\ imp_res_tac inst_clock_neutral_ffi \\ full_simp_tac(srw_ss())[])
+  THEN1 (Cases_on `evaluate (c1,s)` \\ full_simp_tac(srw_ss())[LET_THM] \\ every_case_tac \\ full_simp_tac(srw_ss())[])
+  \\ `get_var_imm ri (s with ffi := c) = get_var_imm ri s` by
          (Cases_on `ri` \\ full_simp_tac(srw_ss())[get_var_imm_def,get_var_def])
   \\ every_case_tac \\ full_simp_tac(srw_ss())[] \\ srw_tac[][] \\ full_simp_tac(srw_ss())[set_var_def]);
 
